src/SepCancel.v
@@ -311,15 +311,9 @@ Module Make (U : SynUnifier) (SH : SepHeap).
       Ordering.list_lex_cmp _ cmp l r.
 
     Definition meta_order_funcs (l r : exprs types * func) : Datatypes.comparison :=
-      match snd l, snd r with
-        | 2, 0 => Datatypes.Lt
-        | 2, 1 => Datatypes.Lt
-        | 2, S (S (S _)) => Datatypes.Lt
-        | _, _ =>
-          match meta_order_args (fst l) (fst r) with
-            | Datatypes.Eq => Compare_dec.nat_compare (snd l) (snd r)
-            | x => x
-          end
+      match meta_order_args (fst l) (fst r) with
+        | Datatypes.Eq => Compare_dec.nat_compare (snd l) (snd r)
+        | x => x
       end.
 
     Definition order_impures (imps : MM.mmap (exprs types)) : cancel_list :=
